examples/preorders/AllocSTwHeaps.fst
@@ -62,7 +62,7 @@ effect IST    (a:Type)
 
 (* A box-like modality for witnessed stable predicates for IST. *)
 
-let ist_witnessed (p:predicate FStar.Heap.heap{stable p heap_rel}) = witnessed #FStar.Heap.heap #heap_rel p
+let ist_witnessed (p:predicate FStar.Heap.heap{stable p heap_rel}) = witnessed heap_rel p
 
 
 (* Generic effects (operations) for IST. *)
